Proofs.v
@@ -1,0 +1,6 @@
+From Licenta Require Import Semantics.
+From Licenta Require Import Syntax.
+From Licenta Require Import Unification_solver.
+
+Check (Sbottom = Prop).
+Check (solver unif_probl1).
