Unification_solver2.v
@@ -1,0 +1,34 @@
+From Licenta Require Import Semantics.
+From Licenta Require Import Syntax.
+
+Require Import String.
+Open Scope string_scope.
+
+Require Import List.
+Import ListNotations.
+
+Definition unification_problem_is_bottom (u : unification_problem) : bool :=
+  true.
+
+Inductive solver : Prop :=
+  | Sbottom (u_p : unification_problem) (H : (unification_problem_is_bottom u_p) = true)
+  | Ssolved (u_p : unification_problem) (H : (unification_problem_in_solved_form u_p) = true)
+  | Sdelete (u_p u_p' : unification_problem)(H : ((term_in_unification_problem u_p term_eq) = true)) (H' : (remove_first_appearance_term_unification_problem u_p term_eq) = u_p')
+  | Sdecompose (u_p u_p' : unification_problem)(tp : term_pair)(H : ((term_in_unification_problem u_p is_decomposition_term_pair) = true)) (H' : (remove_and_replace_decomposition_unif_problem tp u_p) = u_p')
+  | Sorientation (u_p u_p' : unification_problem) (tp : term_pair) (H : ((term_in_unification_problem u_p is_orientation_term_pair) = true)) (H' : (apply_orientation tp u_p) = u_p') 
+  | Selimination (u_p u_p' : unification_problem) (tp : term_pair) (H : ((term_in_unification_problem u_p is_elimination_term_pair) = true)) (H' : (elimination tp u_p) = u_p') 
+  | Sconflict (u_p u_p' : unification_problem) (tp : term_pair) (H : ((term_in_unification_problem u_p is_conflict_term_pair) = true)) (H' : (remove_conflict_term_pair tp u_p) = u_p') 
+  | Soccurs_check (u_p u_p' : unification_problem) (tp : term_pair) (H : ((term_in_unification_problem u_p is_occurs_check_term_pair) = true)) (H' : (occurs_check tp u_p) = u_p').
+
+
+Inductive solver : Type :=
+  | Sbottom (u : unification_problem)
+  | Ssolved (u : unification_problem)
+  | Sdelete (u : unification_problem)
+  | Sdecompose (u : unification_problem)
+  | Sorientation (u : unification_problem)
+  | Selimination (u : unification_problem)
+  | Sconflict (u : unification_problem)
+  | Soccurs_check (u : unification_problem).
+
+Fixpoint 
